theories/Reductions/BMPCP_to_HSC.v
@@ -23,7 +23,7 @@ Import ListNotations.
 Require Import Psatz.
 Require Import ssreflect ssrbool ssrfun. 
 
-From Undecidability Require Import Problems.LPB.
+From Undecidability Require Import Problems.HSC.
 
 Section Facts.
 
@@ -122,11 +122,9 @@ Fixpoint append_word (s: formula) (v: list bool) :=
 Definition encode_word (v: list bool) := append_word bullet v.
 Definition encode_pair (s t: formula) := arr b3 (arr s (arr t b3)).
 
-(*
 Notation "⟨ s , t ⟩" := (encode_pair s t).
 Notation "⟦ v ⟧" := (encode_word v).
 Notation "s → t" := (arr s t) (at level 50).
-*)
 
 (* environment encoding the instance ((v, w), P) of BMPCP *)
 Definition Γ v w P := 
@@ -531,11 +529,361 @@ Proof.
   apply: hsc_var. rewrite /Γ. right. by left.
 Qed.
 
-(* Reduction from BMPCP to LPB and undecidability of LPB *)
+
+(*
+  Proof that there is a fixed Gamma (ΓPCP) with undecidable provability.
+*)
+
+(* fixed type environment encoding PCP *)
+Definition ΓPCP :=
+  [
+    (* ((Q, P), (x, x)) *)
+    encode_pair (var 1) (encode_pair (var 2) (var 2));
+    (* ((P, P), ((x, v'), (y, w'))) → ((((v', w'), Q), P), ((x, •), (y, •))) *)
+    arr 
+      (encode_pair (encode_pair (var 4) (var 4)) (encode_pair (encode_pair (var 5) (var 1)) (encode_pair (var 6) (var 2))))
+      (encode_pair 
+        (encode_pair (encode_pair (encode_pair (var 1) (var 2)) (var 3)) (var 4)) 
+        (encode_pair (encode_pair (var 5) bullet) (encode_pair (var 6) bullet)));
+    (* ((Q, P), (x, y)) → ((((v', w'), Q), P), (x, y)) *)
+    arr 
+      (encode_pair (encode_pair (var 2) (var 3)) (var 4))
+      (encode_pair (encode_pair (encode_pair (var 1) (var 2)) (var 3)) (var 4));
+    (* ((Q, P), ((x, a), v'), y) → ((Q, P), ((x, (a, v')), y) *)
+    arr 
+      (encode_pair (var 1) (encode_pair (encode_pair (encode_pair (var 2) (var 3)) (var 4)) (var 5)))
+      (encode_pair (var 1) (encode_pair (encode_pair (var 2) (encode_pair (var 3) (var 4))) (var 5)));
+    (* ((Q, P), (x, ((y, a), w')) → ((Q, P), (x, (y, (a, w'))) *)
+    arr 
+      (encode_pair (var 1) (encode_pair (var 5) (encode_pair (encode_pair (var 2) (var 3)) (var 4))))
+      (encode_pair (var 1) (encode_pair (var 5) (encode_pair (var 2) (encode_pair (var 3) (var 4)))))
+  ].
+
+
+(* not ΓPCP ⊢ r → r → r *)
+Lemma not_ΓPCP_rrr n r : not (der ΓPCP n (arr r (arr r r))).
+Proof.
+  elim: n r.
+    by move=> ? /der_0E.
+  move=> n IH r /derE => [[ζ [s [k [_ [+ [+]]]]]]].
+  rewrite /ΓPCP /In -/ΓPCP. case; last case; last case; last case; last case; last done.
+  all: move=> <-.
+  case: k => [|k] /=.
+    move=> _. case=> <- _. move /(f_equal size) => /=. by lia.
+  rewrite Forall_norm. by move=> [/IH].
+  all: case: k => [|k] /=.
+  1,3,5,7: by (move=> _; case=> _ <-; move /(f_equal size) => /=; by lia).
+  all: case: k => [|k] /=.
+  1,3,5,7: by (move=> _; case=> <- _; move /(f_equal size) => /=; by lia).
+  all: rewrite ? Forall_norm.
+  all: by move=> [_ [/IH]].
+Qed.
+
+Definition encode_bool b := if b then b2 else b3.
+
+Fixpoint encode_list {X: Type} (encode_X: X -> formula) (A: list X) : formula :=
+  match A with
+  | [] => bullet
+  | a :: A => encode_pair (encode_X a) (encode_list encode_X A)
+  end.
+
+Fixpoint encode_word' (s: formula) (v: list bool) :=
+  match v with
+  | [] => s
+  | a :: v => encode_word' (encode_pair s (if a then b2 else b3)) v
+  end.
+
+Definition encode_word_pair '(x, y) := encode_pair (encode_list encode_bool x) (encode_list encode_bool y).
+
+(* formula encoding the given PCP instance *)
+Definition PCPf P x y := 
+  encode_pair 
+    (encode_pair (encode_list encode_word_pair P) (encode_list encode_word_pair P)) 
+    (encode_pair (encode_pair (encode_word' bullet x) bullet) (encode_pair (encode_word' bullet y) bullet)).
+
+Definition PCPf' Q P s t := 
+    encode_pair 
+      (encode_pair (encode_list encode_word_pair Q) (encode_list encode_word_pair P)) 
+      (encode_pair s t).
+
+Lemma encode_word'_last {x a} : encode_word' bullet (x ++ [a]) = encode_pair (encode_word' bullet x) (encode_bool a).
+Proof.
+  move: (bullet) => s.
+  elim: x s.
+    done.
+  by move=> b x IH s /=.
+Qed.
+
+Lemma hscI {Gamma ζ s t}  : In s Gamma -> t = substitute ζ s -> hsc Gamma t.
+Proof. by move=> /hsc_var + ->. Qed.
+
+
+Lemma ΓPCP_assoc_x {P x r v} : 
+  hsc ΓPCP (PCPf' P P 
+    (encode_pair (encode_word' bullet (x ++ v)) bullet) r) ->
+  hsc ΓPCP (PCPf' P P 
+    (encode_pair (encode_word' bullet x) (encode_list encode_bool v)) r).
+Proof.
+  elim: v x.
+    move=> ?. by rewrite app_nil_r.
+  move=> a v IH x. rewrite -/(app [a] _) app_assoc. move /IH.
+  rewrite encode_word'_last.
+  move /(hsc_arr _ _ _ _). apply.
+  evar (s1 : formula). evar (s2 : formula). evar (s3 : formula). evar (s4 : formula). evar (s5 : formula).
+  pose ζ := 
+    fun i =>
+      match i with
+      | 0 => var 0
+      | 1 => s1 | 2 => s2 | 3 => s3 | 4 => s4 | 5 => s5
+      | _ => var i
+      end.
+  apply: (hscI (ζ := ζ)).
+    rewrite /ΓPCP. do 3 right. left. by reflexivity.
+  rewrite substitute_arrP /PCPf' ? transparent_encode_pair => //=.
+  by rewrite /s1 /s2 /s3 /s4 /s5.
+Qed.
+
+
+Lemma ΓPCP_assoc_y {P r y w} : 
+  hsc ΓPCP (PCPf' P P r 
+    (encode_pair (encode_word' bullet (y ++ w)) bullet)) ->
+  hsc ΓPCP (PCPf' P P r
+    (encode_pair (encode_word' bullet y) (encode_list encode_bool w))).
+Proof.
+  elim: w y.
+    move=> ?. by rewrite app_nil_r.
+  move=> a w IH y. rewrite -/(app [a] _) app_assoc. move /IH.
+  rewrite encode_word'_last.
+  move /(hsc_arr _ _ _ _). apply.
+  evar (s1 : formula). evar (s2 : formula). evar (s3 : formula). evar (s4 : formula). evar (s5 : formula).
+  pose ζ := 
+    fun i =>
+      match i with
+      | 0 => var 0
+      | 1 => s1 | 2 => s2 | 3 => s3 | 4 => s4 | 5 => s5
+      | _ => var i
+      end.
+  apply: (hscI (ζ := ζ)).
+    rewrite /ΓPCP. do 4 right. left. by reflexivity.
+  rewrite substitute_arrP /PCPf' ? transparent_encode_pair => //=.
+  by rewrite /s1 /s2 /s3 /s4 /s5.
+Qed.
+
+
+Lemma ΓPCP_saturate {Q R P s t} : 
+  P = R ++ Q ->
+  hsc ΓPCP (PCPf' Q P s t) ->
+  hsc ΓPCP (PCPf' P P s t).
+Proof.
+  elim /list_last_ind : R Q P.
+    by move=> Q P ->.
+  move=> vw R IH Q P. rewrite -app_assoc. move=> ->.
+  move=> ?. have : hsc ΓPCP (PCPf' ([vw] ++ Q) (R ++ ([vw] ++ Q)) s t).
+    apply: hsc_arr; last eassumption.
+    evar (s1 : formula). evar (s2 : formula). evar (s3 : formula). evar (s4 : formula).
+    pose ζ := 
+      fun i =>
+        match i with
+        | 0 => var 0
+        | 1 => s1 | 2 => s2 | 3 => s3 | 4 => s4
+        | _ => var i
+        end.
+    apply: (hscI (ζ := ζ)).
+      rewrite /ΓPCP. do 2 right. left. by reflexivity.
+    rewrite substitute_arrP /PCPf' ? transparent_encode_pair => //=.
+    by rewrite /s1 /s2 /s3 /s4.
+  move /IH. by apply.
+Qed.
+
+
+Lemma ΓPCP_step {P x y v w} : 
+  In (v, w) P ->
+  hsc ΓPCP (PCPf' P P 
+    (encode_pair (encode_word' bullet x) (encode_list encode_bool v)) 
+    (encode_pair (encode_word' bullet y) (encode_list encode_bool w))) ->
+  hsc ΓPCP (PCPf P x y).
+Proof.
+  move /(@in_split _ _) => [R [Q ?]] ?.
+  have : hsc ΓPCP (PCPf' ((v, w) :: Q) P 
+    (encode_pair (encode_word' bullet x) bullet)
+    (encode_pair (encode_word' bullet y) bullet)).
+    apply: hsc_arr; last eassumption.
+    evar (s1 : formula). evar (s2 : formula). evar (s3 : formula). evar (s4 : formula). evar (s5 : formula). evar (s6 : formula).
+    pose ζ := 
+      fun i =>
+        match i with
+        | 0 => var 0
+        | 1 => s1 | 2 => s2 | 3 => s3 | 4 => s4 | 5 => s5 | 6 => s6
+        | _ => var i
+        end.
+    apply: (hscI (ζ := ζ)).
+      rewrite /ΓPCP. do 1 right. left. by reflexivity.
+    rewrite substitute_arrP /PCPf' ? transparent_encode_pair => //=.
+    by rewrite /s1 /s2 /s3 /s4 /s5 /s6.
+  move /ΓPCP_saturate. apply. by eassumption.
+Qed.
+
+
+Lemma ΓPCP_soundness_ind {v w P A} : 
+  incl A ((v, w) :: P) -> 
+  hsc ΓPCP (PCPf ((v, w) :: P) (v ++ (tau1 A)) (w ++ (tau2 A))) ->
+  hsc ΓPCP (PCPf ((v, w) :: P) v w).
+Proof.
+  elim /list_last_ind : A.
+    move=> _ /=. by rewrite ? app_nil_r.
+  move=> [x y] A IH. rewrite /incl - Forall_forall ? Forall_norm.
+  rewrite Forall_forall -/(incl _ _). move=> [/IH].
+  rewrite tau1_lastP tau2_lastP ? app_assoc.
+  move=> + ? ?; apply.
+  apply: ΓPCP_step; first by eassumption.
+  apply: ΓPCP_assoc_x. apply: ΓPCP_assoc_y.
+  by assumption.
+Qed.
+
+(* if BMPCP has a solution, then the formula (PCPf ((v, w) :: P) v w) is derivable from ΓPCP *)
+Lemma ΓPCP_soundness {v w P} : BMPCP ((v, w), P) -> hsc ΓPCP (PCPf ((v, w) :: P) v w).
+Proof.
+  move=> [A [/ΓPCP_soundness_ind]]. move=> + H.
+  rewrite {}H. apply.
+  evar (s1 : formula). evar (s2 : formula).
+  pose ζ i := 
+    match i with
+    | 0 => var 0 | 1 => s1 | 2 => s2 | _ => var i
+    end.
+  apply: (hscI (ζ := ζ)). by left.
+  rewrite /PCPf transparent_encode_pair => //=.
+  by rewrite /s1 /s2.
+Qed.
+
+Lemma encode_bool_injective {a b} : encode_bool a = encode_bool b -> a = b.
+Proof. case: a b; by case. Qed.
+
+Lemma encode_word'_injective {x y} : encode_word' bullet x = encode_word' bullet y -> x = y.
+Proof.
+  move: x y.
+  elim /list_last_ind => [|a x IHx].
+  all: elim /list_last_ind => [|b y IHy].
+  all: rewrite ? encode_word'_last.
+  all: try done.
+  case. by move /IHx => <- /encode_bool_injective <-.
+Qed.
+
+Lemma encode_list_injective {x y} : encode_list encode_bool x = encode_list encode_bool y -> x = y.
+Proof. 
+  elim: x y=> [|a x IH]; case=> //=.
+  move=> b y. case.
+  by move /encode_bool_injective => <- /IH <-.
+Qed.
+
+Lemma substitute_pairP {ζ s t s' t'} : (substitute ζ (encode_pair s t) = encode_pair s' t') <-> ζ 0 = bullet /\ substitute ζ s = s' /\ substitute ζ t = t'.
+Proof.
+  constructor.
+    by case.
+  by move=> [+ [+ +]] /= => -> -> ->.
+Qed.
+
+
+Lemma ΓPCP_completeness_ind {Q P x y v w n} : incl Q P -> 
+  der ΓPCP n (PCPf' Q P 
+    (encode_pair (encode_word' bullet x) (encode_list encode_bool v))
+    (encode_pair (encode_word' bullet y) (encode_list encode_bool w))) -> 
+  exists A, incl A P /\ x ++ v ++ tau1 A = y ++ w ++ tau2 A.
+Proof.
+  elim: n Q x y v w.
+    by move=> > _ /der_0E.
+  move=> n IH Q x y v w HQ /derE.
+  move=> [ζ [s [k [_ [+ [+]]]]]].
+  have Hu (r) : r = arr r (arr r r) -> False.
+    move /(f_equal size) => /=. by lia.
+  rewrite /ΓPCP /In -/ΓPCP. case; last case; last case; last case; last case; last done.
+  all: move=> <-.
+  case: k=> [|k] /=.
+    move=> _. case. do 7 (move=> _). move=> ->.
+    case=> /encode_word'_injective + /encode_list_injective.
+    move=> -> ->. do 6 (move=> _). by exists [].
+  rewrite ? Forall_norm. by move=> [/not_ΓPCP_rrr].
+  all: case: k=> [|k].
+  1,3,5,7: move=> _ /=; case=> <- *; exfalso; apply: Hu; by eassumption.
+  all: case: k=> [|k].
+  2,4,6,8: move=> /=; rewrite ? Forall_norm; by move=> [_ [/not_ΓPCP_rrr]].
+  all: rewrite substitute_arrP /arguments ? Forall_norm /target.
+  all: move=> Hder.
+  all: rewrite ? substitute_pairP.
+  (* step case *)
+  {
+    move=> [H0] [[_ [H123 H4]]] [_] [[_ [H5 Hv]]] [_ [H6 Hw]].
+    move: H123 HQ. case: Q.
+      done.
+    move=> [v' w'] Q. rewrite /encode_list -/encode_list /encode_word_pair -/encode_word_pair.
+    rewrite ? substitute_pairP.
+    move=> [_ [[_ [H1 H2]] H3]].
+    move: Hder. rewrite ? transparent_encode_pair //.
+    rewrite H1 H2 H4 H5 H6. move /IH. move /(_ ltac:(done)).
+    move=> [A [HAP HxyA]].
+    move /(_ (v', w')). move /(_ ltac:(by left)) => ?.
+    move: Hv Hw. case: v. case: w.
+    move=> _ _.
+    exists ((v', w') :: A). constructor.
+      rewrite /incl - Forall_forall ? Forall_norm Forall_forall. by constructor.
+    by assumption.
+    all: by move=> ? ? /=; rewrite H0.
+  }
+  (* cons case *)
+  {
+    move=> [H0] [[_ [H12 H3]]] H4.
+    move: H12 HQ. case: Q.
+      done.
+    move=> ? Q. rewrite /encode_list -/encode_list ? substitute_pairP. move=> [_ [_ H2]].
+    rewrite /incl -Forall_forall ? Forall_norm Forall_forall.
+    move=> [_ HQ].
+    move: Hder. rewrite ? transparent_encode_pair => //.
+    rewrite H2 H3 H4. move /IH.
+    by apply.
+  }
+  (* assoc x case *)
+  {
+    move=> [H0] [H1] [_] [[_ [H2]]] H34 H5.
+    move: H34. case: v.
+      done.
+    move=> a v. rewrite /encode_list -/encode_list substitute_pairP.
+    move=> [_ [H3 H4]].
+    move: Hder. rewrite ? transparent_encode_pair => //.
+    rewrite H1 H2 H3 H4 H5 -encode_word'_last. move /IH.
+    rewrite -/(app [a] v). move /(_ ltac:(done)) => [A [?]].
+    rewrite - ? app_assoc => ?.
+    by exists A.
+  }
+  (* assoc y case *)
+  {
+    move=> [H0] [H1] [_] [H5] [_ [H2 H34]].
+    move: H34. case: w.
+      done.
+    move=> a w. rewrite /encode_list -/encode_list substitute_pairP.
+    move=> [_ [H3 H4]].
+    move: Hder. rewrite ? transparent_encode_pair => //.
+    rewrite H1 H2 H3 H4 H5 -encode_word'_last. move /IH.
+    rewrite -/(app [a] w). move /(_ ltac:(done)) => [A [?]].
+    rewrite - ? app_assoc => ?.
+    by exists A.
+  }
+Qed.
+
+(* if the formula (PCPf ((v, w) :: P) v w) is derivable from ΓPCP, then BMPCP has a solution *)
+Lemma ΓPCP_completeness {v w P} : hsc ΓPCP (PCPf ((v, w) :: P) v w) -> BMPCP ((v, w), P).
+Proof.
+  move /hsc_der => [n].
+  have -> : PCPf (v / w :: P) v w = 
+    PCPf' (v / w :: P) (v / w :: P) 
+      (encode_pair (encode_word' bullet v) (encode_list encode_bool []))
+      (encode_pair (encode_word' bullet w) (encode_list encode_bool [])) by done.
+  move /ΓPCP_completeness_ind. by apply.
+Qed.
+
+(* Reduction from BMPCP to HSC_AX and undecidability of HSC_AX *)
 
 From Undecidability Require Import Problems.Reduction.
 
-Theorem BMPCP_to_LPB : BMPCP ⪯ LPB.
+Theorem BMPCP_to_HSC_AX : BMPCP ⪯ HSC_AX.
 Proof.
   exists (fun '((v, w), P) => exist _ (Γ v w P) Γ_allowed).
   intros [[v w] P]. constructor.
@@ -543,20 +891,50 @@ Proof.
   exact completeness.
 Qed.
 
-Check BMPCP_to_LPB.
-(* Print Assumptions BMPCP_to_LPB. *)
+Check BMPCP_to_HSC_AX.
+(* Print Assumptions BMPCP_to_HSC_AX. *)
 
 From Undecidability Require Import Problems.TM.
 From Undecidability.PCP Require TM_SRH SRH_SR SR_MPCP MPCP_BMPCP.
 
-Theorem LPB_undec : Halt ⪯ LPB.
+Theorem HSC_AX_undec : Halt ⪯ HSC_AX.
 Proof.
   apply (reduces_transitive TM_SRH.Halt_SRH).
   apply (reduces_transitive SRH_SR.reduction).
   apply (reduces_transitive SR_MPCP.reduction).
   apply (reduces_transitive MPCP_BMPCP.MPCP_to_BMPCP).
-  exact BMPCP_to_LPB.
+  exact BMPCP_to_HSC_AX.
 Qed.
 
-Check LPB_undec.
-(* Print Assumptions LPB_undec. *)
+Check HSC_AX_undec.
+(*Print Assumptions HSC_AX_undec.*)
+
+(* Reduction from BMPCP to HSC_PRV and undecidability of HSC_PRV *)
+
+From Undecidability Require Import Problems.Reduction.
+
+Theorem BMPCP_to_HSC_PRV : BMPCP ⪯ HSC_PRV ΓPCP.
+Proof.
+  exists (fun '((v, w), P) => (PCPf ((v, w) :: P) v w)).
+  intros [[v w] P]. constructor.
+    exact ΓPCP_soundness.
+  exact ΓPCP_completeness.
+Qed.
+
+Check BMPCP_to_HSC_PRV.
+(* Print Assumptions BMPCP_to_HSC_PRV. *)
+
+From Undecidability Require Import Problems.TM.
+From Undecidability.PCP Require TM_SRH SRH_SR SR_MPCP MPCP_BMPCP.
+
+Theorem HSC_PRV_undec : Halt ⪯ HSC_PRV ΓPCP.
+Proof.
+  apply (reduces_transitive TM_SRH.Halt_SRH).
+  apply (reduces_transitive SRH_SR.reduction).
+  apply (reduces_transitive SR_MPCP.reduction).
+  apply (reduces_transitive MPCP_BMPCP.MPCP_to_BMPCP).
+  exact BMPCP_to_HSC_PRV.
+Qed.
+
+Check HSC_PRV_undec.
+(*Print Assumptions HSC_PRV_undec.*)
